Cleanup for thesis

PredicateTermination.thy
@@ -14,7 +14,7 @@ chapter \<open>Predicate Termination\<close>
 (** This inductive definition shows that a predicate relation terminates from some state
     if all successor states in the relation terminate. *)
 inductive trm for r where
-  "(\<forall>b. r a b \<longrightarrow> trm r b) \<Longrightarrow> trm r a"
+  "\<forall>b. r a b \<longrightarrow> trm r b \<Longrightarrow> trm r a"
 
 (** If we have a state that does not have successors in the relation, the relation
     terminates from that state. *)
@@ -28,7 +28,7 @@ lemma trm_final_state:
   "trm r a \<Longrightarrow> \<exists>b. r\<^sup>*\<^sup>* a b \<and> \<not>Domainp r b"
   apply (induction rule: trm.induct)
   apply (simp add: Domainp.simps)
-  using converse_rtranclp_into_rtranclp[of r] by blast
+  using rtranclp_trans[of r] by blast
 
 section \<open>Well-Founded Predicates\<close>
 (** A well-founded predicate relation terminates from any state. *)
@@ -40,11 +40,11 @@ lemma wfP_terminates:
 (** A predicate relation that is well-founded under some invariant that is preserved
     by that relation terminates from any state that satisfies the invariant. *)
 lemma wfP_I_terminates:
-  assumes "I a"
-  assumes "\<And>a b. I a \<Longrightarrow> r a b \<Longrightarrow> I b"
-  assumes "wfP (\<lambda>b a. r a b \<and> I a)"
+  assumes I_init: "I a"
+  assumes I_preserved: "\<And>a b. I a \<Longrightarrow> r a b \<Longrightarrow> I b"
+  assumes wfP_under_I: "wfP (\<lambda>b a. r a b \<and> I a)"
   shows "trm r a"
-  using assms(3,1)
+  using wfP_under_I I_init
   apply (induction rule: wfP_induct_rule)
-  by (blast intro: trm.intros assms(2))
+  by (blast intro: trm.intros I_preserved)
 end
